<?xml version="1.0"?>
<rdf:RDF
    xmlns:tdm="http://ll.mit.edu/2013/ccer/domain/ccer/network/v1/tdm#"
    xmlns:rdf="http://www.w3.org/1999/02/22-rdf-syntax-ns#"
    xmlns:ethernet="http://ll.mit.edu/2013/ccer/domain/ccer/network/v1/ethernet#"
    xmlns:ns="http://www.w3.org/2003/06/sw-vocab-status/ns#"
    xmlns:owl="http://www.w3.org/2002/07/owl#"
    xmlns:dc="http://purl.org/dc/elements/1.1/"
    xmlns:terms="http://purl.org/dc/terms/"
    xmlns:xsd="http://www.w3.org/2001/XMLSchema#"
    xmlns:nml="http://schemas.ogf.org/nml/2013/05/base#"
    xmlns:rdfs="http://www.w3.org/2000/01/rdf-schema#"
    xml:base="http://ll.mit.edu/2013/ccer/domain/ccer/network/v1/tdm">

  <owl:Ontology rdf:about="">
    <owl:versionInfo rdf:datatype="http://www.w3.org/2001/XMLSchema#string"
    >1.0</owl:versionInfo>
    <dc:description xml:lang="en">A vocabulary for defining a TDM network. This schema defines as much as fifteen layers, with STS-3/AUG-1 as the basic Layer, which can actually represent both STS-3 as well as AUG-1. Other important layers are VC-4 / STS-3c SPE, VC-3 / STS-1 SPE and TUG-3. For higher order concatenation, the OC1, OC3, OC12, OC48, OC192 and OC768 layers are defined. For lower order concatenation the layers VT1.5 / VC-11, VT2 / VC-12, VT3, VT6 / VC-2, VT-group / TUG-2 are defined. The layers are highly based on RFC 4606, the GMPLS extensions for GMPLS. This document does not define lower orders than VT1.5. in particular DS0 is not defined, nor the higher order concatenations of DS0: DS1/T1, DS2/T2, DS3/T3, DS4/T4, DS5/T4, E1, E2, E3, E4 and E5. Defining those should be pretty straightforward though, if needed.</dc:description>
    <owl:imports rdf:resource="http://schemas.ogf.org/nml/2013/05/base"/>
    <owl:imports rdf:resource="http://ll.mit.edu/2013/ccer/domain/ccer/network/v1/ethernet"/>
    <rdfs:label>tdm</rdfs:label>
    <ns:term_status>testing</ns:term_status>
    <ns:moreinfo>WARNING: this schema is merely an example what can be done with the layer schema. It was never meant for serious usage. For that, look at the output of the NML workgroup in the OGF (www.ogf.org). We do feel that this schema has a few nice concepts, so feel free to take ideas you like, and put those in your own schema (and let us know you did!). Just don't merely use this schema: it is unmaintained.</ns:moreinfo>
    <owl:imports rdf:resource="http://ll.mit.edu/2013/ccer/domain/ccer/network/v1/atm"/>
    <dc:publisher xml:lang="en">MITT LL in colaboration with IHMC based on ontology developed by  System and Network Engineering group, Universiteit van Amsterdam</dc:publisher>
    <terms:issued rdf:datatype="http://www.w3.org/2001/XMLSchema#string"
    >2013-04-03</terms:issued>
    <dc:title xml:lang="en">Network Markup Language: TDM technologies</dc:title>
    <terms:modified rdf:datatype="http://www.w3.org/2001/XMLSchema#string"
    >2013-04-03</terms:modified>
  </owl:Ontology>

  <owl:Class rdf:ID="STS1-SPENetworkElement">
    <ns:moreinfo>The capacity was not checked in the standard, but taken from a website.</ns:moreinfo>
    <rdfs:comment xml:lang="en">Network Elements on the virtual container (VC)-3 Layer (SDH) or STS-1 SPE (SONET) Layer. The payload of a STS-1 Layer</rdfs:comment>
    <rdfs:label xml:lang="en">STS-1 SPE</rdfs:label>
    <rdfs:subClassOf>
      <owl:Class rdf:about="http://schemas.ogf.org/nml/2013/05/base#NetworkObject"/>
    </rdfs:subClassOf>
  </owl:Class>
  <owl:Class rdf:ID="OC3NetworkElement">
    <ns:moreinfo>The capacity was not checked in the standard, but taken from a website.</ns:moreinfo>
    <rdfs:comment xml:lang="en">Network Elements on the Optical Carrier (OC)-3 Layer.</rdfs:comment>
    <rdfs:label xml:lang="en">OC-3</rdfs:label>
    <rdfs:subClassOf rdf:resource="http://schemas.ogf.org/nml/2013/05/base#NetworkObject"/>
  </owl:Class>
  <owl:Class rdf:ID="OC192NetworkElement">
    <rdfs:comment xml:lang="en">Network Elements on the Optical Carrier (OC)-192 Layer.</rdfs:comment>
    <ns:moreinfo>The capacity was not checked in the standard, but taken from a website.</ns:moreinfo>
    <rdfs:label xml:lang="en">OC-192</rdfs:label>
    <rdfs:subClassOf rdf:resource="http://schemas.ogf.org/nml/2013/05/base#NetworkObject"/>
  </owl:Class>
  <owl:Class rdf:ID="OC768NetworkElement">
    <ns:moreinfo>The capacity was not checked in the standard, but taken from a website.</ns:moreinfo>
    <rdfs:comment xml:lang="en">Network Elements on the Optical Carrier (OC)-768 Layer.</rdfs:comment>
    <rdfs:subClassOf rdf:resource="http://schemas.ogf.org/nml/2013/05/base#NetworkObject"/>
    <rdfs:label xml:lang="en">OC-768</rdfs:label>
  </owl:Class>
  <owl:Class rdf:ID="SLabel">
    <rdfs:subClassOf rdf:resource="http://schemas.ogf.org/nml/2013/05/base#Label"/>
    <rdfs:comment xml:lang="en">Sequence number of a AUG-1 or STS-3 channel (within a STS-n or STM-n) within an optical carrier. This is the same as the "S" label in RFC 4606 (GMPLS). Valid ranges are {1} for OC-3, {1...4} for OC-12, {1...16} for OC-48, {1...64} for OC-192, {1...256} for OC-768, {1...1024} for OC-3072.</rdfs:comment>
    <ns:moreinfo>We now specify the range with XSD (XML schema), but this is not standardised yet. It is likely that the way to specify these limitations (facets) will change. See also "OWL 1.1" and "XML Schema Datatypes in RDF and OWL".</ns:moreinfo>
    <rdfs:label xml:lang="en">S Label</rdfs:label>
  </owl:Class>
  <owl:Class rdf:ID="ULabel">
    <rdfs:subClassOf rdf:resource="http://schemas.ogf.org/nml/2013/05/base#Label"/>
    <rdfs:comment xml:lang="en">Sequence number of a STS-1 SPE (or VC-3) within a STS-3 (or AUG-1). This is the same as the "U" label in RFC 4606 (GMPLS). Valid range is {1...3}.</rdfs:comment>
    <rdfs:label xml:lang="en">U Label</rdfs:label>
    <ns:moreinfo>The range is (1..3). We now specify it with XSD (XML schema), but this is not standardized yet. It is likely that the way to specify these limitations (facets) will change. See also "OWL 1.1" and "XML Schema Datatypes in RDF and OWL".</ns:moreinfo>
  </owl:Class>
  <owl:Class rdf:ID="OC1NetworkElement">
    <ns:moreinfo>The capacity was not checked in the standard, but taken from a website.</ns:moreinfo>
    <rdfs:comment xml:lang="en">Network Elements on the Optical Carrier (OC)-1 Layer.</rdfs:comment>
    <rdfs:label xml:lang="en">OC-1</rdfs:label>
    <rdfs:subClassOf rdf:resource="http://schemas.ogf.org/nml/2013/05/base#NetworkObject"/>
  </owl:Class>
  <owl:Class rdf:ID="KLabel">
    <rdfs:label xml:lang="en">K Label</rdfs:label>
    <rdfs:subClassOf rdf:resource="http://schemas.ogf.org/nml/2013/05/base#Label"/>
    <rdfs:comment xml:lang="en">Sequence number of a TUG-3 within a VC-4. This is the same as the "K" label in RFC 4606 (GMPLS). Valid range is {1...3}.</rdfs:comment>
  </owl:Class>
  <owl:Class rdf:ID="LLabel">
    <rdfs:comment xml:lang="en">Sequence number of a virtual tributary group (VTG) or TUG-2 (Tributary Unit Group) within a STS-1 SPE, VC-3 or TUG-3. This is the same as the "L" label in RFC 4606 (GMPLS). Valid range is {1...7}.</rdfs:comment>
    <rdfs:label xml:lang="en">L Label</rdfs:label>
    <rdfs:subClassOf rdf:resource="http://schemas.ogf.org/nml/2013/05/base#Label"/>
    <ns:moreinfo>The range is (1..7). This probably should be specified. We now specify it with XSD (XML schema), but this is not standardized yet. It is likely that the way to specify these limitations (facets) will change. See also "OWL 1.1" and "XML Schema Datatypes in RDF and OWL".</ns:moreinfo>
  </owl:Class>
  <owl:Class rdf:ID="VT15NetworkElement">
    <ns:moreinfo>The capacity was not checked in the standard, but taken from a website.</ns:moreinfo>
    <rdfs:comment xml:lang="en">Network Elements on the Virtual Tributary (VT)-1.5 or VC-11 Layer.</rdfs:comment>
    <rdfs:label xml:lang="en">VT1.5</rdfs:label>
    <rdfs:subClassOf rdf:resource="http://schemas.ogf.org/nml/2013/05/base#NetworkObject"/>
  </owl:Class>
  <owl:Class rdf:ID="OC12NetworkElement">
    <rdfs:subClassOf rdf:resource="http://schemas.ogf.org/nml/2013/05/base#NetworkObject"/>
    <rdfs:comment xml:lang="en">Network Elements on the Optical Carrier (OC)-12 Layer.</rdfs:comment>
    <ns:moreinfo>The capacity was not checked in the standard, but taken from a website.</ns:moreinfo>
    <rdfs:label xml:lang="en">OC-12</rdfs:label>
  </owl:Class>
  <owl:Class rdf:ID="VC4NetworkElement">
    <ns:moreinfo>The capacity was not checked in the standard, but taken from a website.</ns:moreinfo>
    <rdfs:comment xml:lang="en">Network Elements on the virtual container (VC)-4 Layer (SDH) or STS-3c SPE (SONET) Layer. The payload of a STS-3/AUG-1 Layer</rdfs:comment>
    <rdfs:label xml:lang="en">VC-4</rdfs:label>
    <rdfs:subClassOf rdf:resource="http://schemas.ogf.org/nml/2013/05/base#NetworkObject"/>
  </owl:Class>
  <owl:Class rdf:ID="OC48NetworkElement">
    <ns:moreinfo>The capacity was not checked in the standard, but taken from a website.</ns:moreinfo>
    <rdfs:subClassOf rdf:resource="http://schemas.ogf.org/nml/2013/05/base#NetworkObject"/>
    <rdfs:comment xml:lang="en">Network Elements on the Optical Carrier (OC)-48 Layer.</rdfs:comment>
    <rdfs:label xml:lang="en">OC-48</rdfs:label>
  </owl:Class>
  <owl:Class rdf:ID="OC3072NetworkElement">
    <ns:moreinfo>The capacity was not checked in the standard, but taken from a website.</ns:moreinfo>
    <rdfs:comment xml:lang="en">Network Elements on the Optical Carrier (OC)-3072 Layer.</rdfs:comment>
    <rdfs:label xml:lang="en">OC-3072</rdfs:label>
    <rdfs:subClassOf rdf:resource="http://schemas.ogf.org/nml/2013/05/base#NetworkObject"/>
  </owl:Class>
  <owl:Class rdf:ID="VT2NetworkElement">
    <ns:moreinfo>The capacity was not checked in the standard, but taken from a website.</ns:moreinfo>
    <rdfs:comment xml:lang="en">Network Elements on the Virtual Tributary (VT)-2 or VC-12 Layer.</rdfs:comment>
    <rdfs:label xml:lang="en">VT2</rdfs:label>
    <rdfs:subClassOf rdf:resource="http://schemas.ogf.org/nml/2013/05/base#NetworkObject"/>
  </owl:Class>
  <owl:Class rdf:ID="VT6NetworkElement">
    <ns:moreinfo>The capacity was not checked in the standard, but taken from a website.</ns:moreinfo>
    <rdfs:comment xml:lang="en">Network Elements on the Virtual Tributary (VT)-6 or VC-2 Layer.</rdfs:comment>
    <rdfs:label xml:lang="en">VT6</rdfs:label>
    <rdfs:subClassOf rdf:resource="http://schemas.ogf.org/nml/2013/05/base#NetworkObject"/>
  </owl:Class>
  <owl:Class rdf:ID="TUG3NetworkElement">
    <ns:moreinfo>The capacity was not checked in the standard, but estimated to be roughly the same as a STS-1 capacity; This is the lower limit. This is the upper limit is a STS-1 SPE, but that would mean there are no header bits, which there in fact are.</ns:moreinfo>
    <rdfs:comment xml:lang="en">Network Elements on the Tributary Unit Groups (TUG)-3 Layer (SDH).</rdfs:comment>
    <rdfs:label xml:lang="en">TUG-3</rdfs:label>
    <rdfs:subClassOf rdf:resource="http://schemas.ogf.org/nml/2013/05/base#NetworkObject"/>
  </owl:Class>
  <owl:Class rdf:ID="MLabel">
    <ns:moreinfo>The range is (1..9) or (0/unspecified). We now specify it with XSD (XML schema), but this is not standardized yet. It is likely that the way to specify these limitations (facets) will change. See also "OWL 1.1" and "XML Schema Datatypes in RDF and OWL".</ns:moreinfo>
    <rdfs:comment xml:lang="en">Sequence number of a virtual tributary (VT) in a VT-group (VTG), or the sequence number of a virtual container (VC-11 or VC-12) in a TUG-2 (Tributary Unit Group). The "M" parameters was taken directly from RFC 4606. Valid range is 0..9. 0 indicated a VT-6; 1 or 2 indicate a VT-3; 3, 4 or 5 indicate a VT-2 or VC-12; 6, 7, 8 or 9 indicate a VT-1.5 or VC-11.</rdfs:comment>
    <owl:minCardinality rdf:datatype="http://www.w3.org/2001/XMLSchema#integer"
    >1</owl:minCardinality>
    <xsd:minInclusive rdf:datatype="http://www.w3.org/2001/XMLSchema#integer"
    >0</xsd:minInclusive>
    <rdfs:label xml:lang="en">M Label</rdfs:label>
    <owl:maxCardinality rdf:datatype="http://www.w3.org/2001/XMLSchema#integer"
    >1</owl:maxCardinality>
    <rdfs:subClassOf rdf:resource="http://schemas.ogf.org/nml/2013/05/base#Label"/>
    <xsd:maxInclusive rdf:datatype="http://www.w3.org/2001/XMLSchema#integer"
    >9</xsd:maxInclusive>
  </owl:Class>
  <owl:Class rdf:ID="HierarchyStandard">
    <rdfs:comment xml:lang="en">The Digital Hierarchy standard: SDH or SONET. A STS-3 Interface with "SONET" as the hierarchy is a STS-3. A STS-3 Interface with "SDH" as the hierarchy is a AUG-1 interface.</rdfs:comment>
    <rdfs:label xml:lang="en">Hierarchy</rdfs:label>
  </owl:Class>
  <owl:Class rdf:ID="VT3NetworkElement">
    <ns:moreinfo>The capacity was not checked in the standard, but taken from a website.</ns:moreinfo>
    <rdfs:comment xml:lang="en">Network Elements on the Virtual Tributary (VT)-3 Layer.</rdfs:comment>
    <rdfs:label xml:lang="en">VT3</rdfs:label>
    <rdfs:subClassOf rdf:resource="http://schemas.ogf.org/nml/2013/05/base#NetworkObject"/>
  </owl:Class>
  <owl:Class rdf:ID="VTGNetworkElement">
    <ns:moreinfo>The capacity was not checked in the standard, but taken from a website.</ns:moreinfo>
    <rdfs:comment xml:lang="en">Network Elements on the Virtual Tributary (VT) Group Layer.</rdfs:comment>
    <rdfs:label xml:lang="en">VTG</rdfs:label>
    <rdfs:subClassOf rdf:resource="http://schemas.ogf.org/nml/2013/05/base#NetworkObject"/>
  </owl:Class>
  <owl:Class rdf:about="http://www.w3.org/2001/XMLSchema#integer"/>
  <owl:Class rdf:ID="STS-3NetworkElement">
    <ns:moreinfo>The capacity was not checked in the standard, but taken from a website.</ns:moreinfo>
    <rdfs:comment xml:lang="en">Network Elements on the virtual STS-3 (SONET) or AUG-1 (SDH) Layer. A circuit switched layer, were each link represents a single AUG-1 or (concatenated) STS-3 channel.</rdfs:comment>
    <rdfs:label xml:lang="en">STS-3/AUG-1</rdfs:label>
    <rdfs:subClassOf rdf:resource="http://schemas.ogf.org/nml/2013/05/base#NetworkObject"/>
  </owl:Class>
  <owl:ObjectProperty rdf:ID="tug">
    <rdfs:comment xml:lang="en">The TUG-3 channel. An integer identifying the TUG-3 within a VC-4. This is the same as the "K" label in RFC 4606 (GMPLS). Valid range is {1...3}.</rdfs:comment>
    <rdfs:label xml:lang="en">K</rdfs:label>
    <owl:minCardinality rdf:datatype="http://www.w3.org/2001/XMLSchema#integer"
    >1</owl:minCardinality>
    <owl:maxCardinality rdf:datatype="http://www.w3.org/2001/XMLSchema#integer"
    >1</owl:maxCardinality>
    <rdfs:range rdf:resource="#KLabel"/>
  </owl:ObjectProperty>
  <owl:ObjectProperty rdf:ID="vt3-label">
    <rdfs:range rdf:resource="#MLabel"/>
    <rdfs:label xml:lang="en">M</rdfs:label>
    <owl:maxCardinality rdf:datatype="http://www.w3.org/2001/XMLSchema#integer"
    >1</owl:maxCardinality>
    <owl:minCardinality rdf:datatype="http://www.w3.org/2001/XMLSchema#integer"
    >1</owl:minCardinality>
    <rdfs:comment xml:lang="en">The index of a VT3 channel within a VT group, or equivalently, the index of a VC-2 in a TUG-2. This is the same as the "M" label in RFC 4606 (GMPLS). Valid range is {1...2}.</rdfs:comment>
  </owl:ObjectProperty>
  <owl:ObjectProperty rdf:ID="WANPHY">
    <rdfs:comment xml:lang="en">"Embedding" of WAN PHY (9.5 Gb/s) Ethernet in a OC-192 optical interface. This adaptation encompasses the 10Gbase-W PHY. The Ethernet standard defines different physical media dependent (PMD) adpatations to distinguish between the different underlying wavelengths. While these PMDs are not defined as a specific adaptation, it is possible to distinguish between them by examining the wavelength label of the Lambda layer. This must be 850nm for 10Gbase-SW, 1310nm for 10Gbase-LW and 1550nm for 10Gbase-EW.</rdfs:comment>
    <rdfs:range rdf:resource="http://ll.mit.edu/2013/ccer/domain/ccer/network/v1/ethernet#EthernetNetworkElement"/>
    <rdfs:range rdf:resource="http://schemas.ogf.org/nml/2013/05/base#Port"/>
    <rdfs:label xml:lang="en">WAN PHY</rdfs:label>
  </owl:ObjectProperty>
  <owl:ObjectProperty rdf:ID="STS-in-OC192">
    <rdfs:range rdf:resource="#STS-3NetworkElement"/>
    <rdfs:range rdf:resource="http://schemas.ogf.org/nml/2013/05/base#Port"/>
    <rdfs:label xml:lang="en">STS-3/AUG-1 in OC-192</rdfs:label>
    <rdfs:comment xml:lang="en">Embedding of 192 STS channels or 64 STM channels in a OC-192 optical interface.</rdfs:comment>
  </owl:ObjectProperty>
  <owl:ObjectProperty rdf:ID="VTG-in-STS1-SPE">
    <rdfs:range rdf:resource="#VTGNetworkElement"/>
    <rdfs:range rdf:resource="http://schemas.ogf.org/nml/2013/05/base#Port"/>
    <rdfs:label xml:lang="en">VTG/TUG-2 in STS-1 SPE/VC-3</rdfs:label>
    <rdfs:comment xml:lang="en">Adaptation of 7 Virtual Tributary Groups (VTG) in one STS-1 SPE or, equivalent, 7 TUG-2 in a VC-3.</rdfs:comment>
  </owl:ObjectProperty>
  <owl:ObjectProperty rdf:ID="TUG2-in-TUG3">
    <rdfs:range rdf:resource="http://schemas.ogf.org/nml/2013/05/base#Port"/>
    <rdfs:comment xml:lang="en">Adaptation of 7 Tributary Unit Groups (TUG)-2 in one Tributary Unit Groups (TUG)-3.</rdfs:comment>
    <rdfs:label xml:lang="en">TUG-2 in TUG-3</rdfs:label>
    <rdfs:range rdf:resource="#VTGNetworkElement"/>
  </owl:ObjectProperty>
  <owl:ObjectProperty rdf:ID="STS-in-OC12">
    <rdfs:range rdf:resource="#STS-3NetworkElement"/>
    <rdfs:range rdf:resource="http://schemas.ogf.org/nml/2013/05/base#Port"/>
    <rdfs:label xml:lang="en">STS-3/AUG-1 in OC-12</rdfs:label>
    <rdfs:comment xml:lang="en">Embedding of 12 STS channels or 4 STM channels in a OC-12 optical interface.</rdfs:comment>
  </owl:ObjectProperty>
  <owl:ObjectProperty rdf:ID="VT15-in-VTG">
    <rdfs:range rdf:resource="#VT15NetworkElement"/>
    <rdfs:comment xml:lang="en">Adaptation of 4 VT 1.5 in a VT group or, equivalent, 4 VC-11 in a TUG-2.</rdfs:comment>
    <rdfs:label xml:lang="en">VT1.5 in VTG</rdfs:label>
    <rdfs:range rdf:resource="http://schemas.ogf.org/nml/2013/05/base#Port"/>
  </owl:ObjectProperty>
  <owl:ObjectProperty rdf:ID="vt15-label">
    <rdfs:range rdf:resource="#MLabel"/>
    <rdfs:comment xml:lang="en">The VT1.5 channel within a VT group, or equivalently, the index of a VC-11 in a TUG-2. This is the same as the "M" label in RFC 4606 (GMPLS). Valid range is {6...9}.</rdfs:comment>
    <rdfs:label xml:lang="en">M</rdfs:label>
    <owl:maxCardinality rdf:datatype="http://www.w3.org/2001/XMLSchema#integer"
    >1</owl:maxCardinality>
    <owl:minCardinality rdf:datatype="http://www.w3.org/2001/XMLSchema#integer"
    >1</owl:minCardinality>
  </owl:ObjectProperty>
  <owl:ObjectProperty rdf:ID="vtg">
    <rdfs:range rdf:resource="#LLabel"/>
    <rdfs:comment xml:lang="en">The VTG or TUG-2 channel within a STS-1 SPE, VC-3 or TUG-3. This is the same as the "L" label in RFC 4606 (GMPLS). Valid range is {1...7}.</rdfs:comment>
    <rdfs:label xml:lang="en">L</rdfs:label>
    <owl:maxCardinality rdf:datatype="http://www.w3.org/2001/XMLSchema#integer"
    >1</owl:maxCardinality>
    <owl:minCardinality rdf:datatype="http://www.w3.org/2001/XMLSchema#integer"
    >1</owl:minCardinality>
  </owl:ObjectProperty>
  <owl:ObjectProperty rdf:ID="GiEthernet-in-7-VC4">
    <rdfs:range rdf:resource="http://schemas.ogf.org/nml/2013/05/base#Port"/>
    <ns:moreinfo>WARNING: There is no formal way to specify the order of the 7 VC-4 of a Gigabit Ethernet. A regular layer label would be a good way to do so, but a VC-4 has no label. It is not yet clear if we should provide a regular label for VC-4 for only this purpose, or come up with another concept.</ns:moreinfo>
    <rdfs:range rdf:resource="http://ll.mit.edu/2013/ccer/domain/ccer/network/v1/ethernet#EthernetNetworkElement"/>
    <rdfs:label xml:lang="en">GE in 7 VC-4</rdfs:label>
    <rdfs:comment xml:lang="en">Adaptation of Gigabit Ethernet in 7 VC-4 channels using Generic Framing Procedure for frames (GFP-F).</rdfs:comment>
  </owl:ObjectProperty>
  <owl:ObjectProperty rdf:ID="VT6-in-VTG">
    <rdfs:range rdf:resource="#VT6NetworkElement"/>
    <rdfs:range rdf:resource="http://schemas.ogf.org/nml/2013/05/base#Port"/>
    <rdfs:label xml:lang="en">VT6 in VTG</rdfs:label>
    <rdfs:comment xml:lang="en">Adaptation of a VT 6 in a VT group or, equivalent, a VC-2 in a TUG-2.</rdfs:comment>
  </owl:ObjectProperty>
  <owl:ObjectProperty rdf:ID="TUG3-in-VC4">
    <rdfs:range rdf:resource="http://schemas.ogf.org/nml/2013/05/base#Port"/>
    <rdfs:label xml:lang="en">TUG-3 in VC-4</rdfs:label>
    <rdfs:comment xml:lang="en">Adaptation of 3 TUG-3 in a VC-4.</rdfs:comment>
    <rdfs:range rdf:resource="#TUG3NetworkElement"/>
  </owl:ObjectProperty>
  <owl:ObjectProperty rdf:ID="egresshierarchy">
    <rdfs:comment xml:lang="en">The object Interface is configured to only send out SONET-framed, or SDH-framed channels.</rdfs:comment>
    <rdfs:label xml:lang="en">egress hierarchy</rdfs:label>
    <rdfs:range rdf:resource="#HierarchyStandard"/>
    <rdfs:seeAlso>
      <owl:ObjectProperty rdf:ID="hierarchy"/>
    </rdfs:seeAlso>
  </owl:ObjectProperty>
  <owl:ObjectProperty rdf:ID="STS-in-OC3072">
    <rdfs:range rdf:resource="#STS-3NetworkElement"/>
    <rdfs:range rdf:resource="http://schemas.ogf.org/nml/2013/05/base#Port"/>
    <rdfs:label xml:lang="en">STS-3/AUG-1 in OC-3072</rdfs:label>
    <rdfs:comment xml:lang="en">Embedding of 3072 STS channels or 1024 STM channels in a OC-3072 optical interface.</rdfs:comment>
  </owl:ObjectProperty>
  <owl:ObjectProperty rdf:ID="ingresshierarchy">
    <rdfs:comment xml:lang="en">The object Interface is configured to only accept SONET-framed, or SDH-framed channels. If multiple ingress hierarchy properties are defined, all frames can be accepted at the same time.</rdfs:comment>
    <rdfs:label xml:lang="en">ingress hierarchy</rdfs:label>
    <rdfs:range rdf:resource="#HierarchyStandard"/>
    <rdfs:seeAlso>
      <owl:ObjectProperty rdf:about="#hierarchy"/>
    </rdfs:seeAlso>
  </owl:ObjectProperty>
  <owl:ObjectProperty rdf:ID="VC3-in-AUG1">
    <rdfs:comment xml:lang="en">Adaptation of 3 VC-3 in a AUG-1, or equivalent: 3 STS-1 SPE in a STS-3.</rdfs:comment>
    <rdfs:label xml:lang="en">VC-3/STS-1 in AUG-1/STS-3</rdfs:label>
    <rdfs:range rdf:resource="http://schemas.ogf.org/nml/2013/05/base#Port"/>
    <rdfs:range rdf:resource="#STS1-SPENetworkElement"/>
  </owl:ObjectProperty>
  <owl:ObjectProperty rdf:ID="sts">
    <rdfs:label xml:lang="en">U</rdfs:label>
    <rdfs:comment xml:lang="en">The STS channel. An integer identifying the STS-1 SPE (or VC-3) within a STS-3 (or AUG-1). This is the same as the "U" label in RFC 4606 (GMPLS). Valid range is {1...3}.</rdfs:comment>
    <owl:maxCardinality rdf:datatype="http://www.w3.org/2001/XMLSchema#integer"
    >1</owl:maxCardinality>
    <owl:minCardinality rdf:datatype="http://www.w3.org/2001/XMLSchema#integer"
    >1</owl:minCardinality>
    <rdfs:range rdf:resource="#ULabel"/>
  </owl:ObjectProperty>
  <owl:ObjectProperty rdf:ID="STS-1-SPE-in-OC1">
    <rdfs:range rdf:resource="#STS1-SPENetworkElement"/>
    <rdfs:comment xml:lang="en">Embedding of a STS-1 Synchronous Payload Envelope (SPE) in a OC-1 optical interface.</rdfs:comment>
    <rdfs:label xml:lang="en">STS-1 SPE in OC-1</rdfs:label>
    <rdfs:range rdf:resource="http://schemas.ogf.org/nml/2013/05/base#Port"/>
  </owl:ObjectProperty>
  <owl:ObjectProperty rdf:about="#hierarchy">
    <rdfs:seeAlso rdf:resource="#ingresshierarchy"/>
    <rdfs:comment xml:lang="en">The object Interface is configured to handle either SONET-framed, or SDH-framed channels. The maximum cardinality of this property is 1.</rdfs:comment>
    <rdfs:label xml:lang="en">hierarchy</rdfs:label>
    <rdfs:seeAlso rdf:resource="#egresshierarchy"/>
    <rdfs:range rdf:resource="#HierarchyStandard"/>
  </owl:ObjectProperty>
  <owl:ObjectProperty rdf:ID="VC4-in-AUG1">
    <rdfs:comment xml:lang="en">Adaptation of one VC-4 in a AUG-1, or equivalent: STS-3c SPE in a STS-3.</rdfs:comment>
    <rdfs:label xml:lang="en">VC-4/STS-3c SPE in AUG-1/STS-3</rdfs:label>
    <rdfs:range rdf:resource="http://schemas.ogf.org/nml/2013/05/base#Port"/>
    <rdfs:range rdf:resource="#VC4NetworkElement"/>
  </owl:ObjectProperty>
  <owl:ObjectProperty rdf:ID="STS-in-OC3">
    <rdfs:range rdf:resource="#STS-3NetworkElement"/>
    <rdfs:comment xml:lang="en">Embedding of 3 STS channels (via a STS-3) or 1 STM channel in a OC-3 optical interface.</rdfs:comment>
    <rdfs:label xml:lang="en">STS-3/AUG-1 in OC-3</rdfs:label>
    <rdfs:range rdf:resource="http://schemas.ogf.org/nml/2013/05/base#Port"/>
  </owl:ObjectProperty>
  <owl:ObjectProperty rdf:ID="VT2-in-VTG">
    <rdfs:comment xml:lang="en">Adaptation of 3 VT 2 in a VT group.</rdfs:comment>
    <rdfs:label xml:lang="en">VT2 in VTG</rdfs:label>
    <rdfs:range rdf:resource="http://schemas.ogf.org/nml/2013/05/base#Port"/>
    <rdfs:range rdf:resource="#VT2NetworkElement"/>
  </owl:ObjectProperty>
  <owl:ObjectProperty rdf:ID="GiEthernet-in-8-VC4">
    <rdfs:comment xml:lang="en">Adaptation of Gigabit Ethernet in 8 VC-4 channels using a proprietary standard used by some Cisco devices.</rdfs:comment>
    <ns:moreinfo>WARNING: There is no formal way to specify the order of the 8 VC-4 of a Gigabit Ethernet. A regular layer label would be a good way to do so, but a VC-4 has no label. It is not yet clear if we should provide a regular label for VC-4 for only this purpose, or come up with another concept.</ns:moreinfo>
    <rdfs:label xml:lang="en">GE in 8 VC-4</rdfs:label>
    <rdfs:range rdf:resource="http://schemas.ogf.org/nml/2013/05/base#Port"/>
    <rdfs:range rdf:resource="http://ll.mit.edu/2013/ccer/domain/ccer/network/v1/ethernet#EthernetNetworkElement"/>
  </owl:ObjectProperty>
  <owl:ObjectProperty rdf:ID="STS-in-OC48">
    <rdfs:range rdf:resource="#STS-3NetworkElement"/>
    <rdfs:range rdf:resource="http://schemas.ogf.org/nml/2013/05/base#Port"/>
    <rdfs:label xml:lang="en">STS-3/AUG-1 in OC-48</rdfs:label>
    <rdfs:comment xml:lang="en">Embedding of 48 STS channels or 16 STM channels in a OC-48 optical interface.</rdfs:comment>
  </owl:ObjectProperty>
  <owl:ObjectProperty rdf:ID="stm">
    <rdfs:label xml:lang="en">S</rdfs:label>
    <rdfs:comment xml:lang="en">The STM channel. An integer identifying the AUG-1 or STS-3 channel (within a STS-n or STM-n) within an optical carrier. This is the same as the "S" label in RFC 4606 (GMPLS). Valid ranges are {1} for OC-3, {1...4} for OC-12, {1...16} for OC-48, {1...64} for OC-192, {1...256} for OC-768</rdfs:comment>
    <owl:maxCardinality rdf:datatype="http://www.w3.org/2001/XMLSchema#integer"
    >1</owl:maxCardinality>
    <owl:minCardinality rdf:datatype="http://www.w3.org/2001/XMLSchema#integer"
    >1</owl:minCardinality>
    <rdfs:range rdf:resource="#SLabel"/>
  </owl:ObjectProperty>
  <owl:ObjectProperty rdf:ID="STS-in-OC768">
    <rdfs:range rdf:resource="#STS-3NetworkElement"/>
    <rdfs:range rdf:resource="http://schemas.ogf.org/nml/2013/05/base#Port"/>
    <rdfs:label xml:lang="en">STS-3/AUG-1 in OC-768</rdfs:label>
    <rdfs:comment xml:lang="en">Embedding of 768 STS channels or 256 STM channels in a OC-768 optical interface.</rdfs:comment>
  </owl:ObjectProperty>
  <owl:ObjectProperty rdf:ID="vt2-label">
    <rdfs:range rdf:resource="#MLabel"/>
    <rdfs:label xml:lang="en">M</rdfs:label>
    <owl:maxCardinality rdf:datatype="http://www.w3.org/2001/XMLSchema#integer"
    >1</owl:maxCardinality>
    <owl:minCardinality rdf:datatype="http://www.w3.org/2001/XMLSchema#integer"
    >1</owl:minCardinality>
    <rdfs:comment xml:lang="en">The VT2 channel within a VT group, or equivalently, the index of a VC-12 in a TUG-2. This is the same as the "M" label in RFC 4606 (GMPLS). Valid range is {3...5}.</rdfs:comment>
  </owl:ObjectProperty>
  <owl:ObjectProperty rdf:ID="VT3-in-VTG">
    <rdfs:range rdf:resource="#VT3NetworkElement"/>
    <rdfs:comment xml:lang="en">Adaptation of 2 VT 3 in a VT group or, equivalent, 2 VC-12 in a TUG-2.</rdfs:comment>
    <rdfs:label xml:lang="en">VT3 in VTG</rdfs:label>
    <rdfs:range rdf:resource="http://schemas.ogf.org/nml/2013/05/base#Port"/>
  </owl:ObjectProperty>
  <owl:ObjectProperty rdf:ID="ATM-in-16-VC4">
    <rdfs:comment xml:lang="en">Adaptation of ATM in a VC-4-16c.</rdfs:comment>
    <rdfs:range rdf:resource="http://ll.mit.edu/2013/ccer/domain/ccer/network/v1/atm#ATMNetworkElement"/>
    <ns:moreinfo>WARNING: There is no formal way to specify the order of the 16 VC-4 of this ATM link. A regular layer label would be a good way to do so, but a VC-4 has no label. It is not yet clear if we should provide a regular label for VC-4 for only this purpose, or come up with another concept.</ns:moreinfo>
    <rdfs:label xml:lang="en">ATM in 16 VC-4</rdfs:label>
    <rdfs:range rdf:resource="http://schemas.ogf.org/nml/2013/05/base#Port"/>
  </owl:ObjectProperty>
  <tdm:HierarchyStandard rdf:ID="SONET">
    <rdfs:label xml:lang="en">SONET</rdfs:label>
    <rdfs:comment xml:lang="en">The ANSI SONET standards.</rdfs:comment>
  </tdm:HierarchyStandard>
  <owl:AnnotationProperty rdf:about="http://www.w3.org/2002/07/owl#versionInfo"/>
  <tdm:HierarchyStandard rdf:ID="SDH">
    <rdfs:label xml:lang="en">SDH</rdfs:label>
    <rdfs:comment xml:lang="en">The ITU SDH standards.</rdfs:comment>
  </tdm:HierarchyStandard>
</rdf:RDF>

<!-- Created with TopBraid -->
