<?xml version="1.0"?>
<rdf:RDF
    xmlns:vpn="http://ll.mit.edu/2013/ccer/domain/ccer/network/v1/vpn#"
    xmlns:rdf="http://www.w3.org/1999/02/22-rdf-syntax-ns#"
    xmlns:ns="http://www.w3.org/2003/06/sw-vocab-status/ns#"
    xmlns:owl="http://www.w3.org/2002/07/owl#"
    xmlns:dc="http://purl.org/dc/elements/1.1/"
    xmlns:terms="http://purl.org/dc/terms/"
    xmlns:xsd="http://www.w3.org/2001/XMLSchema#"
    xmlns:nml="http://schemas.ogf.org/nml/2013/05/base#"
    xmlns:rdfs="http://www.w3.org/2000/01/rdf-schema#"
  xml:base="http://ll.mit.edu/2013/ccer/domain/ccer/network/v1/vpn">
  <owl:Ontology rdf:about="">
    <owl:imports rdf:resource="http://schemas.ogf.org/nml/2013/05/base"/>
    <dc:publisher xml:lang="en">MITT LL in colaboration with IHMC based on System and Network Engineering group, Universiteit van Amsterdam</dc:publisher>
    <dc:description xml:lang="en">A vocabulary for defining PPP links, L2TP tunnels and MPLS paths. Of these layers, only the MPLS layer has a label: the mplsLabel. PPP and L2TP are single link-only technologies. The ad-hoc combination of these three technologies in a single schema leads to the correct observation that this schema can be considered a bit immature. The naming is a bit odd: VPN, while only L2TP really is a tunneling protocol.</dc:description>
    <dc:title xml:lang="en">Network Markup Language: PPP, L2TP and MPLS technologies</dc:title>
    <terms:issued rdf:datatype="http://www.w3.org/2001/XMLSchema#string"
    >2013-03-24</terms:issued>
    <rdfs:label>vpn</rdfs:label>
    <terms:modified rdf:datatype="http://www.w3.org/2001/XMLSchema#string"
    >2013-03-24</terms:modified>
    <owl:versionInfo rdf:datatype="http://www.w3.org/2001/XMLSchema#string"
    >1.0</owl:versionInfo>
    <ns:term_status>testing</ns:term_status>
  </owl:Ontology>
  <owl:Class rdf:ID="L2TPInterface">
    <rdfs:subClassOf rdf:resource="http://schemas.ogf.org/nml/2013/05/base#Port"/>
    <rdfs:label xml:lang="en">L2TP</rdfs:label>
    <rdfs:subClassOf>
      <owl:Class rdf:ID="L2TPNetworkElement"/>
    </rdfs:subClassOf>
  </owl:Class>
  <owl:Class rdf:ID="MPLSNetworkElement">
    <rdfs:subClassOf rdf:resource="http://schemas.ogf.org/nml/2013/05/base#NetworkObject"/>
    <rdfs:comment xml:lang="en">Network Elements on the MPLS Layer. Each packet consists of one or more MPLS labels, followed by a payload. Note that labels in labels are NOT represented as MPLS in MPLS.</rdfs:comment>
    <rdfs:label xml:lang="en">MPLS</rdfs:label>
  </owl:Class>
  <owl:Class rdf:ID="PPPInterface">
    <rdfs:subClassOf rdf:resource="http://schemas.ogf.org/nml/2013/05/base#Port"/>
    <rdfs:label xml:lang="en">PPP</rdfs:label>
    <rdfs:subClassOf>
      <owl:Class rdf:ID="PPPNetworkElement"/>
    </rdfs:subClassOf>
  </owl:Class>
  <owl:Class rdf:about="#PPPNetworkElement">
    <rdfs:subClassOf rdf:resource="http://schemas.ogf.org/nml/2013/05/base#NetworkObject"/>
    <rdfs:comment xml:lang="en">Network Elements on the Point-to-Point Protocol (PPP) Layer, as defined in RFC 1661. PPP only defines links, and has no switching labels. A PPP packet consists of a 1-byte or 2-byte protocol header, followed by a variable payload.</rdfs:comment>
    <rdfs:label xml:lang="en">PPP</rdfs:label>
  </owl:Class>
  <owl:Class rdf:ID="MPLSInterface">
    <rdfs:subClassOf rdf:resource="#MPLSNetworkElement"/>
    <rdfs:subClassOf rdf:resource="http://schemas.ogf.org/nml/2013/05/base#Port"/>
    <rdfs:label xml:lang="en">MPLS</rdfs:label>
  </owl:Class>
  <owl:Class rdf:about="http://www.w3.org/2001/XMLSchema#integer"/>
  <owl:Class rdf:ID="MPLSLabel">
    <rdfs:label xml:lang="en">MPLS Label</rdfs:label>
    <rdfs:subClassOf rdf:resource="http://schemas.ogf.org/nml/2013/05/base#Label"/>
    <rdfs:comment xml:lang="en">Value of the label field in the MPLS header. This is the topmost label, thus the label of the current link.</rdfs:comment>
  </owl:Class>
  <owl:Class rdf:about="#L2TPNetworkElement">
    <rdfs:subClassOf rdf:resource="http://schemas.ogf.org/nml/2013/05/base#NetworkObject"/>
    <rdfs:comment xml:lang="en">Network Elements on the Layer 2 Tunneling Protocol (L2TP) Layer, as defined in RFC 3931. L2TP only defines links, and has no switching labels.</rdfs:comment>
    <rdfs:label xml:lang="en">L2TP</rdfs:label>
  </owl:Class>
  <owl:ObjectProperty rdf:ID="mplsLabel">
    <rdfs:range rdf:resource="#MPLSLabel"/>
    <rdfs:label xml:lang="en">label</rdfs:label>
    <rdfs:comment xml:lang="en">The topmost label in a MPLS packet. The MPLS label is a 20-bit integer.</rdfs:comment>
    <owl:maxCardinality rdf:datatype="http://www.w3.org/2001/XMLSchema#integer"
    >1</owl:maxCardinality>
    <owl:minCardinality rdf:datatype="http://www.w3.org/2001/XMLSchema#integer"
    >1</owl:minCardinality>
  </owl:ObjectProperty>
  <owl:ObjectProperty rdf:ID="ethernet-in-L2TP">
    <rdfs:range rdf:resource="http://schemas.ogf.org/nml/2013/05/base#Port"/>
    <rdfs:comment xml:lang="en">Adaptation of Ethernet in L2TP by creating an Ethernet Port Pseudowire as defined by RFC 4719.</rdfs:comment>
    <rdfs:label xml:lang="en">Ethernet in L2TP</rdfs:label>
    <rdfs:range rdf:resource="http://ll.mit.edu/2013/ccer/domain/ccer/network/v1/ethernet#EthernetNetworkElement"/>
  </owl:ObjectProperty>
  <owl:ObjectProperty rdf:ID="atm-in-L2TP">
    <rdfs:range rdf:resource="http://schemas.ogf.org/nml/2013/05/base#Port"/>
    <rdfs:comment xml:lang="en">Adaptation of ATM in L2TP by creating an AAL5-SDU Mode Pseudowire as defined by RFC 4454.</rdfs:comment>
    <rdfs:label xml:lang="en">ATM in L2TP</rdfs:label>
    <rdfs:range rdf:resource="http://ll.mit.edu/2013/ccer/domain/ccer/network/v1/atm#ATMNetworkElement"/>
  </owl:ObjectProperty>
  <owl:ObjectProperty rdf:ID="ppp-in-L2TP">
    <rdfs:range rdf:resource="#PPPInterface"/>
    <rdfs:comment xml:lang="en">Adaptation of PPP in L2TP by creating a HDLC Pseudorwire as defined by RFC 4349.</rdfs:comment>
    <rdfs:label xml:lang="en">PPP in L2TP</rdfs:label>
  </owl:ObjectProperty>
  <owl:ObjectProperty rdf:ID="ip-in-PPP">
    <rdfs:range rdf:resource="http://schemas.ogf.org/nml/2013/05/base#Port"/>
    <rdfs:comment xml:lang="en">A simple adaptation embedding IP packets 1:1 in the payload of PPP packets. The protocol field is set to 0x0021 (for IPv4) or 0x0057 (for IPv6), as defined by www.iana.org/assignments/ppp-numbers.</rdfs:comment>
    <rdfs:label xml:lang="en">IP in PPP</rdfs:label>
    <rdfs:range rdf:resource="http://ll.mit.edu/2013/ccer/domain/ccer/network/v1/ip#IPNetworkElement"/>
  </owl:ObjectProperty>
  <owl:ObjectProperty rdf:ID="ip-in-MPLS">
    <rdfs:range rdf:resource="http://schemas.ogf.org/nml/2013/05/base#Port"/>
    <rdfs:comment xml:lang="en">A simple adaptation embedding IP packets in the payload of a MPLS packet.</rdfs:comment>
    <rdfs:label xml:lang="en">IP in MPLS</rdfs:label>
    <rdfs:range rdf:resource="http://ll.mit.edu/2013/ccer/domain/ccer/network/v1/ip#IPNetworkElement"/>
  </owl:ObjectProperty>
  <owl:ObjectProperty rdf:ID="l2tp-in-MPLS">
    <rdfs:range rdf:resource="#L2TPInterface"/>
    <rdfs:comment xml:lang="en">A simple adaptation embedding L2TP packets in the payload of a MPLS packet.</rdfs:comment>
    <rdfs:label xml:lang="en">L2TP in MPLS</rdfs:label>
  </owl:ObjectProperty>
</rdf:RDF>

<!-- Created with TopBraid -->
