<?xml version="1.0"?>
<rdf:RDF
    xmlns:physical="http://ll.mit.edu/2013/ccer/domain/ccer/network/v1/physical#"
    xmlns:ethernet="http://ll.mit.edu/2013/ccer/domain/ccer/network/v1/ethernet#"
    xmlns:bundle="http://ll.mit.edu/2013/ccer/domain/ccer/network/v1/bundle#"
    xmlns:atm="http://ll.mit.edu/2013/ccer/domain/ccer/network/v1/atm#"
    xmlns:dc="http://purl.org/dc/elements/1.1/"
    xmlns:wdm="http://ll.mit.edu/2013/ccer/domain/ccer/network/v1/wdm#"
    xmlns:nml="http://schemas.ogf.org/nml/2013/05/base#"
    xmlns:tdm="http://ll.mit.edu/2013/ccer/domain/ccer/network/v1/tdm#"
    xmlns:rdf="http://www.w3.org/1999/02/22-rdf-syntax-ns#"
    xmlns:ns="http://www.w3.org/2003/06/sw-vocab-status/ns#"
    xmlns:owl="http://www.w3.org/2002/07/owl#"
    xmlns:terms="http://purl.org/dc/terms/"
    xmlns:xsd="http://www.w3.org/2001/XMLSchema#"
    xmlns:rdfs="http://www.w3.org/2000/01/rdf-schema#"
  xml:base="http://ll.mit.edu/2013/ccer/domain/ccer/network/v1/wdm">
  <owl:Ontology rdf:about="">
    <ns:term_status>testing</ns:term_status>
    <rdfs:label>wdm</rdfs:label>
    <owl:versionInfo rdf:datatype="http://www.w3.org/2001/XMLSchema#string"
    >1.0</owl:versionInfo>
    <owl:imports rdf:resource="http://schemas.ogf.org/nml/2013/05/base"/>
    <dc:description xml:lang="en">A vocabulary for defining an wavelength division multiplexing (WDM) network. This schema defines two layers: Lambda the layer representing individual wavelengths, and the Fiber layer representing the collection of wavelengths on a fiber. Note that all higher layers like Ethernet and OC-channels are defined over a Lambda, rather than directly over Fiber. The reason is that for nearly all Something-over-Fiber adaptations, it is trivial to adapt it over a specific Lambda as well, by simply buying a GBIC, SFP, XFP or other pluggable laser for a specific wavelength. This schema does not define a separate layer for wavelength groups. It that is to be added, it should go between the Lambda and Fiber layer. The spacing property of the Fiber Interface defines what type of Lambda is transmitted over the fiber: a single Lambda, CWDM, DWDM (with 100, 50, 25 or 12.5 GHz spacing). Different spacings lead to incompatibilities between interfaces. The model is not always ideal to describe a fiber network as only has a sketchy concept of power levels and power loss.</dc:description>
    <owl:imports rdf:resource="http://ll.mit.edu/2013/ccer/domain/ccer/network/v1/tdm"/>
    <owl:imports rdf:resource="http://ll.mit.edu/2013/ccer/domain/ccer/network/v1/bundle"/>
    <ns:moreinfo>WARNING: this schema is merely an example what can be done with the layer schema. It was never meant for serious usage. For that, look at the output of the NML workgroup in the OGF (www.ogf.org). We do feel that this schema has a few nice concepts, so feel free to take ideas you like, and put those in your own schema (and let us know you did!). Just don't merely use this schema: it is unmaintained.</ns:moreinfo>
    <dc:publisher xml:lang="en">MITT LL in colaboration with IHMC based on ontology developed by System and Network Engineering group, Universiteit van Amsterdam</dc:publisher>
    <terms:issued rdf:datatype="http://www.w3.org/2001/XMLSchema#string"
    >2013-04-03</terms:issued>
    <dc:title xml:lang="en">Network Markup Language: WDM and Fiber technologies</dc:title>
    <owl:imports rdf:resource="http://ll.mit.edu/2013/ccer/domain/ccer/network/v1/atm"/>
    <owl:imports rdf:resource="http://ll.mit.edu/2013/ccer/domain/ccer/network/v1/ethernet"/>
    <terms:modified rdf:datatype="http://www.w3.org/2001/XMLSchema#string"
    >2013-04-03</terms:modified>
  </owl:Ontology>
  <owl:Class rdf:ID="TransceiverType">
    <rdfs:label xml:lang="en">Transceiver</rdfs:label>
    <rdfs:comment xml:lang="en">A pluggable transceiver type.</rdfs:comment>
  </owl:Class>
  <owl:Class rdf:ID="SpacingDistance">
    <rdfs:label xml:lang="en">Spacing</rdfs:label>
    <rdfs:comment xml:lang="en">A spacing between individual wavelengths.</rdfs:comment>
  </owl:Class>
  <owl:Class rdf:ID="ConnectorType">
    <rdfs:label xml:lang="en">Connector</rdfs:label>
    <rdfs:comment xml:lang="en">A type of connector.</rdfs:comment>
  </owl:Class>
  <owl:Class rdf:ID="CladdingType">
    <rdfs:label xml:lang="en">Cladding</rdfs:label>
    <rdfs:comment xml:lang="en">The diameter of the core and cladding of a fiber.</rdfs:comment>
  </owl:Class>
  <owl:Class rdf:ID="FiberNetworkElement">
    <rdfs:comment xml:lang="en">Network Elements on the Fiber Layer. A circuit switched layer.</rdfs:comment>
    <rdfs:subClassOf rdf:resource="http://schemas.ogf.org/nml/2013/05/base#NetworkObject"/>
    <rdfs:label xml:lang="en">Fiber</rdfs:label>
  </owl:Class>
  <owl:Class rdf:ID="LambdaNetworkElement">
    <rdfs:label xml:lang="en">Lambda</rdfs:label>
    <rdfs:subClassOf rdf:resource="http://schemas.ogf.org/nml/2013/05/base#NetworkObject"/>
    <rdfs:comment xml:lang="en">Network Elements on the Lambda Layer. A link on this layer represents an individual wavelength in a WDM network.</rdfs:comment>
  </owl:Class>
  <owl:Class rdf:ID="PolishType">
    <rdfs:label xml:lang="en">Polish</rdfs:label>
    <rdfs:comment xml:lang="en">A polish or cut type of a connector</rdfs:comment>
  </owl:Class>
  <owl:ObjectProperty rdf:ID="WDM">
    <rdfs:comment xml:lang="en">Wavelength Division Multiplexing (WDM): embedding of one or more wavelengths in a fiber.</rdfs:comment>
    <rdfs:range rdf:resource="http://schemas.ogf.org/nml/2013/05/base#Port"/>
    <rdfs:label xml:lang="en">WDM</rdfs:label>
    <rdfs:range rdf:resource="#LambdaNetworkElement"/>
  </owl:ObjectProperty>
  <owl:ObjectProperty rdf:ID="eth10base-F">
    <rdfs:range rdf:resource="http://ll.mit.edu/2013/ccer/domain/ccer/network/v1/ethernet#EthernetNetworkElement"/>
    <rdfs:range rdf:resource="http://schemas.ogf.org/nml/2013/05/base#Port"/>
    <rdfs:label xml:lang="en">10base-F</rdfs:label>
    <rdfs:comment xml:lang="en">Adaptation of 10 Mb/s Ethernet into a single wavelength. This includes the 10base-FL (full duplex), 10base-FB and 10base-FP Ethernet PMDs. The encoding is 4b/5b with Manchester pulsing. This adaptation MUST go over multimode fiber and MUST have a wavelength of 850nm.</rdfs:comment>
  </owl:ObjectProperty>
  <owl:ObjectProperty rdf:ID="oc1-in-Lambda">
    <rdfs:range rdf:resource="http://ll.mit.edu/2013/ccer/domain/ccer/network/v1/tdm#OC1NetworkElement"/>
    <rdfs:range rdf:resource="http://schemas.ogf.org/nml/2013/05/base#Port"/>
    <rdfs:label xml:lang="en">OC-1 in Lambda</rdfs:label>
    <rdfs:comment xml:lang="en">OC-1 embedded in a Lambda, using 64b/66b encoding, with standard Non-Return-to-Zero (NRZ) pulsing.</rdfs:comment>
  </owl:ObjectProperty>
  <owl:ObjectProperty rdf:ID="cladding">
    <rdfs:range rdf:resource="#CladdingType"/>
    <rdfs:label xml:lang="en">cladding</rdfs:label>
    <rdfs:comment xml:lang="en">The cladding of a fiber, describing the diameter of the core and the cladding of a fiber. Possible values include multi mode and single mode fiber.</rdfs:comment>
  </owl:ObjectProperty>
  <owl:ObjectProperty rdf:ID="eth10Gbase-R">
    <rdfs:range rdf:resource="http://ll.mit.edu/2013/ccer/domain/ccer/network/v1/ethernet#EthernetNetworkElement"/>
    <rdfs:range rdf:resource="http://schemas.ogf.org/nml/2013/05/base#Port"/>
    <rdfs:label xml:lang="en">10Gbase-R</rdfs:label>
    <rdfs:comment xml:lang="en">Adaptation of 10 Gb/s Ethernet into a single wavelength. This includes the all 10Gbase-R Ethernet PMDs, including the non-standard 10Gbase-ZR. The encoding is 8b/10b with Non-Return-to-Zero (NRZ) pulsing. For 10Gbase-SR the fiber MUST be multi mode and the wavelength MUST be 850nm. For 10Gbase-LR the fiber MUST be single mode and the wavelength MUST be 1310nm. For 10Gbase-ER the fiber MUST be single mode and the wavelength MUST be 1550nm. For 10Gbase-ZR the fiber MUST be single mode and the wavelength MUST be 1550nm.</rdfs:comment>
  </owl:ObjectProperty>
  <owl:ObjectProperty rdf:ID="transceiver">
    <rdfs:comment xml:lang="en">The transceiver property described the type of pluggable interface in the physical fiber interface. Possible values include GBIC, SFP, XFP, X2, XENPAK and XPAK.</rdfs:comment>
    <rdfs:label xml:lang="en">transceiver</rdfs:label>
    <rdfs:range rdf:resource="#TransceiverType"/>
  </owl:ObjectProperty>
  <owl:ObjectProperty rdf:ID="oc768-in-Lambda">
    <rdfs:range rdf:resource="http://ll.mit.edu/2013/ccer/domain/ccer/network/v1/tdm#OC768NetworkElement"/>
    <rdfs:comment xml:lang="en">OC-768 embedded in a Lambda, using 64b/66b encoding, with standard Non-Return-to-Zero (NRZ) pulsing.</rdfs:comment>
    <rdfs:label xml:lang="en">OC-768 in Lambda</rdfs:label>
    <rdfs:range rdf:resource="http://schemas.ogf.org/nml/2013/05/base#Port"/>
  </owl:ObjectProperty>
  <owl:ObjectProperty rdf:ID="oc3-in-Lambda">
    <rdfs:range rdf:resource="http://ll.mit.edu/2013/ccer/domain/ccer/network/v1/tdm#OC3NetworkElement"/>
    <rdfs:range rdf:resource="http://schemas.ogf.org/nml/2013/05/base#Port"/>
    <rdfs:label xml:lang="en">OC-3 in Lambda</rdfs:label>
    <rdfs:comment xml:lang="en">OC-3 embedded in a Lambda, using 64b/66b encoding, with standard Non-Return-to-Zero (NRZ) pulsing.</rdfs:comment>
  </owl:ObjectProperty>
  <owl:ObjectProperty rdf:ID="oc192-in-Lambda">
    <rdfs:range rdf:resource="http://ll.mit.edu/2013/ccer/domain/ccer/network/v1/tdm#OC192NetworkElement"/>
    <rdfs:comment xml:lang="en">OC-192 embedded in a Lambda, using 64b/66b encoding, with standard Non-Return-to-Zero (NRZ) pulsing.</rdfs:comment>
    <rdfs:label xml:lang="en">OC-192 in Lambda</rdfs:label>
    <rdfs:range rdf:resource="http://schemas.ogf.org/nml/2013/05/base#Port"/>
  </owl:ObjectProperty>
  <owl:ObjectProperty rdf:ID="eth1000base-X">
    <rdfs:range rdf:resource="http://ll.mit.edu/2013/ccer/domain/ccer/network/v1/ethernet#EthernetNetworkElement"/>
    <rdfs:comment xml:lang="en">Adaptation of 1000 Mb/s Ethernet into a single wavelength. This includes the all 1000base-X Ethernet PMDs, including the non-standard 1000base-ZX. The encoding is 8b/10b with Non-Return-to-Zero (NRZ) pulsing. For 1000base-SX the fiber MUST be multi mode and the wavelength label MUST be 850nm (actual wavelength between 770nm and 860nm). For 1000base-LX the fiber can be either multi mode or single mode and the wavelength label MUST be 1310nm (actual wavelength between 1270nm and 1355nm). For 1000base-ZX (=1000base-LH) the fiber MUST be single mode and the wavelength MUST be 1310nm.</rdfs:comment>
    <rdfs:label xml:lang="en">1000base-X</rdfs:label>
    <rdfs:range rdf:resource="http://schemas.ogf.org/nml/2013/05/base#Port"/>
  </owl:ObjectProperty>
  <owl:ObjectProperty rdf:ID="strand">
    <rdfs:range rdf:resource="http://ll.mit.edu/2013/ccer/domain/ccer/network/v1/bundle#StrandLabel"/>
    <owl:minCardinality rdf:datatype="http://www.w3.org/2001/XMLSchema#integer"
    >0</owl:minCardinality>
    <owl:maxCardinality rdf:datatype="http://www.w3.org/2001/XMLSchema#integer"
    >1</owl:maxCardinality>
    <rdfs:label xml:lang="en">strand</rdfs:label>
    <rdfs:comment xml:lang="en">The identification number of a certain fiber within a bundle of links.</rdfs:comment>
  </owl:ObjectProperty>
  <owl:ObjectProperty rdf:ID="wavelength">
    <owl:minCardinality rdf:datatype="http://www.w3.org/2001/XMLSchema#integer"
    >1</owl:minCardinality>
    <owl:maxCardinality rdf:datatype="http://www.w3.org/2001/XMLSchema#integer"
    >1</owl:maxCardinality>
    <rdfs:range>
      <rdf:Description rdf:about="http://ll.mit.edu/2013/ccer/domain/ccer/network/v1/wdm#WavelengthLabel">
        <ns:moreinfo>The range of this variable depends on the "Spacing" parameter in the Fiber layer. All valid values should probably be specified somehow. Perhaps in a long list using RDF:Alt. See for now the wdm:SpacingDistance descriptions for valid values. Plus 1300.00nm for 100base-FX</ns:moreinfo>
        <rdfs:comment xml:lang="en">The wavelength (?) in nanometer of a "Lamba" Link over a wavelength division multiplexing (WDM) system. Basically the colour of a laser. The accuracy must be sufficient for the given spacing, and considering that two floats are compared by at least 20 significant bits (6 decimal places).</rdfs:comment>
        <rdfs:subClassOf rdf:resource="http://schemas.ogf.org/nml/2013/05/base#Label"/>
        <rdfs:label xml:lang="en">Wavelength</rdfs:label>
      </rdf:Description>
    </rdfs:range>
    <rdfs:label xml:lang="en">wavelength</rdfs:label>
    <rdfs:comment xml:lang="en">The wavelength label, specifying wavelength (?) of a lambda in nanometers. The range of wavelengths is a float, representing the wavelength through vacuum in nanometers. To compare if two wavelengths are equal, at least the 6 most significant bits must be compared, and two literals with a decimal representation must be the same if it is logically the same.</rdfs:comment>
  </owl:ObjectProperty>
  <owl:ObjectProperty rdf:ID="eth100base-FX">
    <rdfs:range rdf:resource="http://ll.mit.edu/2013/ccer/domain/ccer/network/v1/ethernet#EthernetNetworkElement"/>
    <rdfs:comment xml:lang="en">Adaptation of 100 Mb/s Ethernet into a single wavelength using the 100base-FX PMD. The encoding is 4b/5b with Non-Return-to-Zero Inverted (NRZI) pulsing. This adaptation MUST go over multi mode fiber (not single mode!) and MUST have a wavelength of 1300nm.</rdfs:comment>
    <rdfs:label xml:lang="en">100base-FX</rdfs:label>
    <rdfs:range rdf:resource="http://schemas.ogf.org/nml/2013/05/base#Port"/>
  </owl:ObjectProperty>
  <owl:ObjectProperty rdf:ID="oc48-in-Lambda">
    <rdfs:range rdf:resource="http://ll.mit.edu/2013/ccer/domain/ccer/network/v1/tdm#OC48NetworkElement"/>
    <rdfs:range rdf:resource="http://schemas.ogf.org/nml/2013/05/base#Port"/>
    <rdfs:label xml:lang="en">OC-48 in Lambda</rdfs:label>
    <rdfs:comment xml:lang="en">OC-48 embedded in a Lambda, using 64b/66b encoding, with standard Non-Return-to-Zero (NRZ) pulsing.</rdfs:comment>
  </owl:ObjectProperty>
  <owl:ObjectProperty rdf:ID="spacing">
    <rdfs:comment xml:lang="en">The spacing in GHz between two wavelengths. Possible values include 100 GHz, 50GHz, but also CWDM (20nm), WWDM (only a few wavelengths possible) or single lambda (only one wavelength possible).</rdfs:comment>
    <rdfs:label xml:lang="en">spacing</rdfs:label>
    <rdfs:range rdf:resource="#SpacingDistance"/>
  </owl:ObjectProperty>
  <owl:ObjectProperty rdf:ID="polish">
    <rdfs:range rdf:resource="#PolishType"/>
    <rdfs:label xml:lang="en">polish</rdfs:label>
    <rdfs:comment xml:lang="en">The polish property describes the type of physical contact between the fiber core and cladding. Typically, this is a plain "physical contact" (PC), but other fiber cuts, like angled physical contact (APC) have the advantage of having less reflection.</rdfs:comment>
  </owl:ObjectProperty>
  <owl:ObjectProperty rdf:ID="atm-in-Lambda">
    <rdfs:range rdf:resource="http://ll.mit.edu/2013/ccer/domain/ccer/network/v1/atm#ATMNetworkElement"/>
    <rdfs:range rdf:resource="http://schemas.ogf.org/nml/2013/05/base#Port"/>
    <rdfs:label xml:lang="en">ATM in Lambda</rdfs:label>
    <rdfs:comment xml:lang="en">Adaptation of 155 Mb/s ATM over a single Lambda.</rdfs:comment>
  </owl:ObjectProperty>
  <owl:ObjectProperty rdf:ID="connector">
    <rdfs:comment xml:lang="en">The type of connector. The interface is always female, and the connected to link is always male. If it is the other way around, that must be clearly specified in the connector type.</rdfs:comment>
    <rdfs:label xml:lang="en">connector type</rdfs:label>
    <rdfs:range rdf:resource="#ConnectorType"/>
  </owl:ObjectProperty>
  <owl:DatatypeProperty rdf:ID="egressPowerLevel">
    <rdfs:comment xml:lang="en">The egress power level describes the power level as send out by a fiber interface to each connected to interface. The power level is measured in dBm, where 0 dBm equals 1 milliWatt of power. The maximum cardinality of this property is 1.</rdfs:comment>
    <rdfs:range rdf:resource="http://www.w3.org/2001/XMLSchema#float"/>
    <rdfs:label xml:lang="en">egress power level</rdfs:label>
  </owl:DatatypeProperty>
  <owl:DatatypeProperty rdf:ID="ingressPowerLevel">
    <rdfs:comment xml:lang="en">The ingress power level defines the maximum power level received by a fiber interface coming from interfaces connected to here. The power level is measured in dBm, where 0 dBm equals 1 milliWatt of power. The maximum cardinality of this property is 1.</rdfs:comment>
    <rdfs:range rdf:resource="http://www.w3.org/2001/XMLSchema#float"/>
    <rdfs:label xml:lang="en">ingress power level</rdfs:label>
  </owl:DatatypeProperty>
  <owl:DatatypeProperty rdf:ID="powerLoss">
    <rdfs:comment xml:lang="en">The power loss that is to be expected when light travels through a network element. For a link, the powerloss property of the Link resource, and the powerloss of the two Interface resources (if any) must be added up. The power loss is measured in dB. The maximum cardinality of this property is 1.</rdfs:comment>
    <rdfs:range rdf:resource="http://www.w3.org/2001/XMLSchema#float"/>
    <rdfs:label xml:lang="en">power loss</rdfs:label>
  </owl:DatatypeProperty>
  <wdm:SpacingDistance rdf:ID="SingleLambda">
    <rdfs:label xml:lang="en">only a single Lambda can be carried</rdfs:label>
    <rdfs:comment xml:lang="en">Only a single Lambda can be carried over the fiber.</rdfs:comment>
  </wdm:SpacingDistance>
  <wdm:SpacingDistance rdf:ID="spacing100GHz">
    <rdfs:comment xml:lang="en">Dense Wavelength Division Multiplexing (DWDM) with a central frequency of 193.1THz and a spacing of 100GHz between different wavelengths, as defined in ITU G.694.1. The associated wavelength are the wavelengths in vacuum.</rdfs:comment>
    <rdfs:label xml:lang="en">100GHz</rdfs:label>
  </wdm:SpacingDistance>
  <wdm:SpacingDistance rdf:ID="WWDM-bands">
    <rdfs:comment xml:lang="en">Only a single Lambda can be carried in each band: O, E, S, C, L and U band. The O (Original) band at 1260nm - 1360nm; the E (Extended) band at 1360nm - 1460nm; the S (Short) band at 1460nm - 1530nm; the C (Conventional) band at 1530nm - 1565nm; the L (Long) band at 1565nm - 1625nm; and the U (Ultra-long) band at 1625nm - 1675nm. The values to be used as wavelength label are: 1310, 1410, 1490, 1550, 1590 and 1650.</rdfs:comment>
    <rdfs:label xml:lang="en">6 WWDM bands</rdfs:label>
  </wdm:SpacingDistance>
  <wdm:SpacingDistance rdf:ID="spacing12.5GHz">
    <rdfs:comment xml:lang="en">Dense Wavelength Division Multiplexing (DWDM) with a central frequency of 193.1THz and a spacing of 12.5GHz between different wavelengths, as defined in ITU G.694.1. The associated wavelength are the wavelengths in vacuum.</rdfs:comment>
    <rdfs:label xml:lang="en">12.5GHz</rdfs:label>
  </wdm:SpacingDistance>
  <wdm:TransceiverType rdf:ID="XENPAK">
    <rdfs:label xml:lang="en">XENPAK</rdfs:label>
    <rdfs:comment xml:lang="en">XENPAK pluggable transceiver for 10 Gb/s interfaces</rdfs:comment>
  </wdm:TransceiverType>
  <wdm:CladdingType rdf:ID="SingleMode">
    <rdfs:comment xml:lang="en">Single mode fiber: a fiber with a core between 3?m and 10?m (typically 8.3?m) and a cladding of 125?m diameter. Single mode fiber can support DWDM, and is often used in conjunction with wavelengths in the 1300nm - 1600nm range.</rdfs:comment>
    <rdfs:label xml:lang="en">SM</rdfs:label>
  </wdm:CladdingType>
  <wdm:TransceiverType rdf:ID="XPAK">
    <rdfs:label xml:lang="en">XPAK</rdfs:label>
    <rdfs:comment xml:lang="en">XPAK pluggable transceiver for 10 Gb/s interfaces</rdfs:comment>
  </wdm:TransceiverType>
  <rdf:Description rdf:about="http://ll.mit.edu/2013/ccer/domain/ccer/network/v1/wdm#GBIC">
    <rdfs:label xml:lang="en">GBIC</rdfs:label>
    <rdfs:comment xml:lang="en">GBIC pluggable transceiver for 1000 Mb/s interfaces</rdfs:comment>
  </rdf:Description>
  <wdm:PolishType rdf:ID="UPC">
    <rdfs:label xml:lang="en">UPC</rdfs:label>
    <rdfs:comment xml:lang="en">Ultra Physical Contact (UPC) polish</rdfs:comment>
  </wdm:PolishType>
  <wdm:ConnectorType rdf:ID="SC-Connector">
    <rdfs:label xml:lang="en">SC</rdfs:label>
    <rdfs:comment xml:lang="en">SC connector</rdfs:comment>
  </wdm:ConnectorType>
  <wdm:SpacingDistance rdf:ID="spacing25GHz">
    <rdfs:label xml:lang="en">25GHz</rdfs:label>
    <rdfs:comment xml:lang="en">Dense Wavelength Division Multiplexing (DWDM) with a central frequency of 193.1THz and a spacing of 25GHz between different wavelengths, as defined in ITU G.694.1. The associated wavelength are the wavelengths in vacuum.</rdfs:comment>
  </wdm:SpacingDistance>
  <wdm:PolishType rdf:ID="SPC">
    <rdfs:label xml:lang="en">SPC</rdfs:label>
    <rdfs:comment xml:lang="en">Super Physical Contact (SPC) polish</rdfs:comment>
  </wdm:PolishType>
  <rdf:Description rdf:ID="FiberNetworkElement">
    <rdfs:subClassOf rdf:resource="http://schemas.ogf.org/nml/2013/05/base#NetworkObject"/>
  </rdf:Description>
  <wdm:TransceiverType rdf:ID="SFP">
    <rdfs:comment xml:lang="en">SFP pluggable transceiver for 1000 Mb/s interfaces</rdfs:comment>
    <rdfs:label xml:lang="en">SFP</rdfs:label>
  </wdm:TransceiverType>
  <wdm:CladdingType rdf:ID="MultiMode">
    <rdfs:comment xml:lang="en">Multi mode fiber: a fiber with a core of 50?m or 62.5?m and a cladding of 125?m diameter. Multi mode fiber is useful to transport wavelengths around 850nm, though it can be used for 1310nm for short distances.</rdfs:comment>
    <rdfs:label xml:lang="en">MM</rdfs:label>
  </wdm:CladdingType>
  <wdm:SpacingDistance rdf:ID="spacing50GHz">
    <rdfs:label xml:lang="en">50GHz</rdfs:label>
    <rdfs:comment xml:lang="en">Dense Wavelength Division Multiplexing (DWDM) with a central frequency of 193.1THz and a spacing of 50GHz between different wavelengths, as defined in ITU G.694.1. The associated wavelength are the wavelengths in vacuum.</rdfs:comment>
  </wdm:SpacingDistance>
  <wdm:PolishType rdf:ID="APC">
    <rdfs:label xml:lang="en">APC</rdfs:label>
    <rdfs:comment xml:lang="en">Angled Physical Contact (APC) polish</rdfs:comment>
  </wdm:PolishType>
  <wdm:SpacingDistance rdf:ID="WWDM-windows">
    <rdfs:comment xml:lang="en">Only a single Lambda can be carried in each optical window: 850nm, 1310nm, and 1550nm.</rdfs:comment>
    <rdfs:label xml:lang="en">3 WWDM windows</rdfs:label>
  </wdm:SpacingDistance>
  <wdm:TransceiverType rdf:ID="XFP">
    <rdfs:label xml:lang="en">XFP</rdfs:label>
    <rdfs:comment xml:lang="en">XFP pluggable transceiver for 10 Gb/s interfaces</rdfs:comment>
  </wdm:TransceiverType>
  <wdm:ConnectorType rdf:ID="ST-Connector">
    <rdfs:label xml:lang="en">ST</rdfs:label>
    <rdfs:comment xml:lang="en">Straight Tip (ST) connector</rdfs:comment>
  </wdm:ConnectorType>
  <wdm:SpacingDistance rdf:ID="CWDM">
    <rdfs:comment xml:lang="en">Coarse Wavelength Division Multiplexing (CWDM) as defined in ITU G.694.2. A spacing of 20nm, with a starting frequency of 1271nm, going up to 1611nm, and beyond. Note that not all frequencies may be used due to the water peak.</rdfs:comment>
    <rdfs:label xml:lang="en">CWDM</rdfs:label>
  </wdm:SpacingDistance>
  <wdm:ConnectorType rdf:ID="FC-Connector">
    <rdfs:label xml:lang="en">FC</rdfs:label>
    <rdfs:comment xml:lang="en">FC connector</rdfs:comment>
  </wdm:ConnectorType>
  <wdm:ConnectorType rdf:ID="LC-Connector">
    <rdfs:label xml:lang="en">LC</rdfs:label>
    <rdfs:comment xml:lang="en">LC connector</rdfs:comment>
  </wdm:ConnectorType>
  <wdm:PolishType rdf:ID="PC">
    <rdfs:label xml:lang="en">PC</rdfs:label>
    <rdfs:comment xml:lang="en">Physical Contact (PC) polish</rdfs:comment>
  </wdm:PolishType>
  <wdm:TransceiverType rdf:ID="X2">
    <rdfs:label xml:lang="en">X2</rdfs:label>
    <rdfs:comment xml:lang="en">X2 pluggable transceiver for 10 Gb/s interfaces</rdfs:comment>
  </wdm:TransceiverType>
</rdf:RDF>

<!-- Created with TopBraid -->
