<?xml version="1.0"?>
<rdf:RDF
    xmlns:rdf="http://www.w3.org/1999/02/22-rdf-syntax-ns#"
    xmlns:ethernet="http://ll.mit.edu/2013/ccer/domain/ccer/network/v1/ethernet#"
    xmlns:wireless="http://ll.mit.edu/2013/ccer/domain/ccer/network/v1/wireless#"
    xmlns:ns="http://www.w3.org/2003/06/sw-vocab-status/ns#"
    xmlns:owl="http://www.w3.org/2002/07/owl#"
    xmlns:dc="http://purl.org/dc/elements/1.1/"
    xmlns:terms="http://purl.org/dc/terms/"
    xmlns:xsd="http://www.w3.org/2001/XMLSchema#"
    xmlns:nml="http://schemas.ogf.org/nml/2013/05/base#"
    xmlns:rdfs="http://www.w3.org/2000/01/rdf-schema#"
  xml:base="http://ll.mit.edu/2013/ccer/domain/ccer/network/v1/wireless">
  <owl:Ontology rdf:about="">
    <rdfs:label>wireless</rdfs:label>
    <dc:description xml:lang="en">A vocabulary for defining a wireless network. This schema only defines the 802.11 layer. It could easily be extended to support other wireless layers.</dc:description>
    <terms:issued rdf:datatype="http://www.w3.org/2001/XMLSchema#string"
    >2013-03-27</terms:issued>
    <owl:imports rdf:resource="http://schemas.ogf.org/nml/2013/05/base"/>
    <terms:modified rdf:datatype="http://www.w3.org/2001/XMLSchema#string"
    >2007-03-27</terms:modified>
    <dc:publisher xml:lang="en">MITT LL in colaboration with IHMC based on ontology developed by  System and Network Engineering group, Universiteit van Amsterdam</dc:publisher>
    <owl:versionInfo rdf:datatype="http://www.w3.org/2001/XMLSchema#string"
    >1.0</owl:versionInfo>
    <dc:title xml:lang="en">Network Markup Language: Wireless technologies</dc:title>
    <ns:term_status>testing</ns:term_status>
  </owl:Ontology>
  <owl:Class rdf:ID="IEEE802-11Standard">
    <rdfs:comment xml:lang="en">The shielding of the wireless pairs in a cable.</rdfs:comment>
    <rdfs:label xml:lang="en">Shielding</rdfs:label>
  </owl:Class>
  <owl:Class rdf:ID="AccessSecurity">
    <rdfs:comment xml:lang="en">The encryption used to authenticate to a base station.</rdfs:comment>
    <rdfs:label xml:lang="en">AccessSecurity</rdfs:label>
  </owl:Class>
  <owl:Class rdf:ID="SSIDLabel">
    <rdfs:subClassOf rdf:resource="http://schemas.ogf.org/nml/2013/05/base#Label"/>
    <rdfs:label xml:lang="en">SSID</rdfs:label>
    <rdfs:comment xml:lang="en">The service set identifier (SSID), identifying packets on a wireless network to belong to a certain network. The SSID is a case-senstive string of up to 32 alphanumeric characters. Since xsd:string is also case-senstive, we can simply use the XML string comparison.</rdfs:comment>
    <ns:moreinfo>The range is a 32-char alphanumeric case-sensitive string. This should be specified. Perhaps using OWL 1.1 or XSD facets. However, neither is standardized yet.</ns:moreinfo>
  </owl:Class>
  <owl:Class rdf:ID="IEEE802-11NetworkElement">
    <rdfs:subClassOf rdf:resource="http://schemas.ogf.org/nml/2013/05/base#NetworkObject"/>
    <rdfs:label xml:lang="en">802.11</rdfs:label>
    <rdfs:comment xml:lang="en">Network Elements on the 802.11 Layer. This encompasses all 802.11 standards. This layer is modeled a packet switched broadcast network, much like TaggedEthernet, and has the SSID as the basic switching label. The modeling does not fit well, as it only has a rudimentary concept of signal strengths. This could probably be improved by creating two layers: one for each SSID, and one for each pair of transmitter and receiver.</rdfs:comment>
  </owl:Class>
  <owl:ObjectProperty rdf:ID="Ethernet-in-802-11">
    <rdfs:label xml:lang="en">Ethernet in 802.11</rdfs:label>
    <rdfs:range rdf:resource="http://schemas.ogf.org/nml/2013/05/base#Port"/>
    <rdfs:comment xml:lang="en">Adaptation of Ethernet in a specific SSID.</rdfs:comment>
  </owl:ObjectProperty>
  <owl:ObjectProperty rdf:ID="standard">
    <rdfs:range rdf:resource="#IEEE802-11Standard"/>
    <rdfs:comment xml:lang="en">The wireless standard used in the SSID network.</rdfs:comment>
    <rdfs:label xml:lang="en">standard</rdfs:label>
  </owl:ObjectProperty>
  <owl:ObjectProperty rdf:ID="ssid">
    <rdfs:comment xml:lang="en">The service set identifier (SSID), identifying packets on a wireless network to belong to a certain network. The SSID is a case-senstive string of up to 32 alphanumeric characters.</rdfs:comment>
    <rdfs:label xml:lang="en">SSID</rdfs:label>
    <owl:minCardinality rdf:datatype="http://www.w3.org/2001/XMLSchema#integer"
    >0</owl:minCardinality>
    <owl:maxCardinality rdf:datatype="http://www.w3.org/2001/XMLSchema#integer"
    >1</owl:maxCardinality>
    <rdfs:range rdf:resource="#SSIDLabel"/>
  </owl:ObjectProperty>
  <owl:ObjectProperty rdf:ID="encryption">
    <rdfs:range rdf:resource="#AccessSecurity"/>
    <rdfs:comment xml:lang="en">The standard describing the initial authentication and key exchange used on a wireless network.</rdfs:comment>
    <rdfs:label xml:lang="en">encryption</rdfs:label>
  </owl:ObjectProperty>
  <owl:DatatypeProperty rdf:ID="frequency">
    <rdfs:label xml:lang="en">frequency</rdfs:label>
    <rdfs:range rdf:resource="http://www.w3.org/2001/XMLSchema#float"/>
    <rdfs:comment xml:lang="en">The central frequency of the channel at which an Interface operates, in Hz. For 802.11g, allowed values are 2412E6, 2417E6, 2422E6, 2427E6, 2432E6, 2437E6, 2442E6, 2447E6, 2452E6, 2457E6, 2462E6, 2467E6, 2472E6. Other standards have other frequencies.</rdfs:comment>
  </owl:DatatypeProperty>
  <wireless:AccessSecurity rdf:ID="WPA">
    <rdfs:comment xml:lang="en">Wi-Fi Protected Access(WPA). WPA uses the RC4 stream cipher.</rdfs:comment>
    <rdfs:label xml:lang="en">WPA</rdfs:label>
  </wireless:AccessSecurity>
  <wireless:IEEE802-11Standard rdf:ID="IEEE802-11b">
    <rdfs:comment xml:lang="en">IEEE 802.11b standard. 802.11b operates between 2.4 an 2.5 GHz, and has a maximum data rate of 11 Mb/s.</rdfs:comment>
    <rdfs:label xml:lang="en">802.11b</rdfs:label>
  </wireless:IEEE802-11Standard>
  <wireless:IEEE802-11Standard rdf:ID="IEEE802-11a">
    <rdfs:comment xml:lang="en">IEEE 802.11a standard. 802.11a operates between 5.1 an 5.9 GHz, and has a maximum data rate of 54 Mb/s. Due to the high frequency, it does not easily penetrate walls.</rdfs:comment>
    <rdfs:label xml:lang="en">802.11a</rdfs:label>
  </wireless:IEEE802-11Standard>
  <wireless:IEEE802-11Standard rdf:ID="IEEE802-11n">
    <rdfs:label xml:lang="en">802.11n</rdfs:label>
    <rdfs:comment xml:lang="en">IEEE 802.11n standard. 802.11n operates at the 2.4 GHz or 5 GHz bands, and has a maximum data rate of 540 Mb/s.</rdfs:comment>
  </wireless:IEEE802-11Standard>
  <wireless:AccessSecurity rdf:ID="WEP">
    <rdfs:label xml:lang="en">WEP</rdfs:label>
    <rdfs:comment xml:lang="en">Wired Equivalent Privacy (WEP). WEP uses the RC4 stream cipher.</rdfs:comment>
  </wireless:AccessSecurity>
  <wireless:IEEE802-11Standard rdf:ID="IEEE802-11g">
    <rdfs:label xml:lang="en">802.11g</rdfs:label>
    <rdfs:comment xml:lang="en">IEEE 802.11g standard. 802.11g operates between 2.4 and 2.5 GHz, and has a maximum data rate of 54 Mb/s.</rdfs:comment>
  </wireless:IEEE802-11Standard>
  <wireless:AccessSecurity rdf:ID="WPA2">
    <rdfs:label xml:lang="en">WPA2</rdfs:label>
    <rdfs:comment xml:lang="en">IEEE 802.11i access encryption, also known as WPA2. WPA2 uses the AES block cipher.</rdfs:comment>
  </wireless:AccessSecurity>
</rdf:RDF>

<!-- Created with TopBraid -->
